fix types mismatch with calloc

src/Primitive/Boolean/VstDec.v
@@ -31,12 +31,12 @@ Definition bool_ber_decode_spec : ident * funspec :=
                 Vint (Int.repr tag_mode))
       GLOBALS ()
       SEP (valid_pointer bv_p;
-          (* if eq_dec bv_p nullval 
+          if eq_dec bv_p nullval 
            then emp
-           else data_at_ Tsh tint bv_p ; *)
+           else data_at_ Tsh tint bv_p ; 
            data_at Tsh asn_codec_ctx_s ctx ctx_p;
            data_at_ Tsh type_descriptor_s td_p;
-           data_at Tsh (tarray tuchar (Zlength buf)) (map Vbyte buf) buf_p;
+           data_at Tsh (tarray tuchar (Zlength buf)) (map Vubyte buf) buf_p;
            data_at Tsh (tptr tvoid) bv_p bv_pp;
            data_at_ Tsh asn_dec_rval_s res_p)
     POST [tvoid] 
@@ -47,21 +47,21 @@ Definition bool_ber_decode_spec : ident * funspec :=
          valid_pointer bv_p;
          data_at Tsh asn_codec_ctx_s ctx ctx_p;
          data_at_ Tsh type_descriptor_s td_p;
-         data_at Tsh (tarray tuchar (Zlength buf)) (map Vbyte buf) buf_p;
+         data_at Tsh (tarray tuchar (Zlength buf)) (map Vubyte buf) buf_p;
          (* Changed according to spec *)
          let RC_FAIL := data_at Tsh asn_dec_rval_s (Vint (Int.repr 2), Vzero) res_p in
          if eq_dec bv_p nullval 
-         then EX v : val, EX t : type, EX ls : list byte, 
+         then EX v : val, EX ls : list int, 
                      data_at Tsh (tptr tvoid) v bv_pp *
                      if eq_dec v nullval 
                      then RC_FAIL  
                      else match bool_decoder td buf with
                            | Some (r, c) => 
                              data_at Tsh asn_dec_rval_s (Vzero, Vint (Int.repr c)) res_p *
-                             data_at Tsh tschar (Val.of_bool r) v
+                             data_at Tsh tint (Val.of_bool r) v
                            | None => RC_FAIL * 
-                                    malloc_token Ews t v *
-                                    data_at Ews (tarray tschar 1) (map Vbyte ls) v 
+                                    (* malloc_token Ews (tarray tuchar 1) v * *)
+                                    data_at Ews (tarray tint 1) (map Vint ls) v 
                                     
       
                           end
@@ -69,8 +69,8 @@ Definition bool_ber_decode_spec : ident * funspec :=
               match bool_decoder td buf with
                 | Some (r, c) => 
                   data_at Tsh asn_dec_rval_s (Vzero, Vint (Int.repr c)) res_p *
-                  data_at Tsh tschar (Val.of_bool r) bv_p 
-                | None => RC_FAIL
+                  data_at Tsh tint (Val.of_bool r) bv_p 
+                | None => RC_FAIL * data_at_ Tsh tint bv_p
                 end).
 
 
@@ -80,8 +80,10 @@ Definition Gprog := ltac:(with_library prog [(_calloc, calloc_spec);
 
 Definition if_post1  bv_p v__res__1 v_tmp_error v_length v_rval 
            res_p ctx ctx_p td_p bv_pp buf buf_p size tag_mode := 
-  EX p : val, EX t : type, EX ls : list byte,
-  PROP (if eq_dec bv_p nullval then p <> nullval else (p = bv_p /\ bv_p <> nullval))
+  EX p : val, EX ls : list int,
+  PROP (if eq_dec bv_p nullval 
+        then p <> nullval /\ Zlength ls = 1
+        else (p = bv_p /\ bv_p <> nullval))
   LOCAL (temp _st p; 
          temp _t'11 bv_p;
          lvar __res__1 (Tstruct _asn_dec_rval_s noattr) v__res__1;
@@ -98,12 +100,12 @@ Definition if_post1  bv_p v__res__1 v_tmp_error v_length v_rval
        data_at_ Tsh (Tstruct _asn_dec_rval_s noattr) v_rval; valid_pointer bv_p;
        data_at Tsh asn_codec_ctx_s ctx ctx_p;
        data_at_ Tsh type_descriptor_s td_p;
-       data_at Tsh (tarray tuchar (Zlength buf)) (map Vbyte buf) buf_p;
+       data_at Tsh (tarray tuchar (Zlength buf)) (map Vubyte buf) buf_p;
        data_at Tsh (tptr tvoid) p bv_pp;
        if eq_dec bv_p nullval 
-       then data_at_ Tsh asn_dec_rval_s res_p * malloc_token Ews t p * 
-            data_at Ews (tarray tschar 1) (map Vbyte ls) p 
-       else data_at_ Tsh asn_dec_rval_s res_p 
+       then data_at_ Tsh asn_dec_rval_s res_p * (* malloc_token Ews (tarray tuchar 1) p * *) 
+            data_at Ews (tarray tint 1) (map Vint ls) p 
+       else data_at_ Tsh asn_dec_rval_s res_p * data_at_ Tsh tint bv_p
        ).
 Ltac forward_empty_loop :=
       match goal with
@@ -111,6 +113,251 @@ Ltac forward_empty_loop :=
           forward_loop Pre break: Pre; try forward ; try entailer! 
       end. 
 
+Theorem bool_der_encode : semax_body Vprog Gprog 
+           (normalize_function f_BOOLEAN_decode_ber composites) 
+           bool_ber_decode_spec.
+Proof.
+  start_function.
+  break_if. 
+  - (* bv = nullval *)
+  rename H0 into DT.
+  rename H1 into Size.
+  rename H2 into Len.
+  repeat forward.
+  forward_if (if_post1 bv_p v__res__1 v_tmp_error v_length v_rval res_p ctx 
+                       ctx_p td_p bv_pp buf buf_p size tag_mode).
+  * (* _st = NULL *)
+    forward_call (1, sizeof tint, tint).
+    cbn; nia.
+    Intros p.
+    repeat forward.
+    forward_if.
+    {
+      if_tac; break_let; 
+      cbn in H19; subst; entailer!. }
+    -- (* malloc returned null *)
+      unfold abbreviate in POSTCONDITION.
+      unfold fst in *; rewrite H3 in *. 
+      rewrite if_true in * by reflexivity.
+      repeat forward.
+      entailer!.
+      Exists nullval (snd p).
+      rewrite if_true by assumption.
+      entailer!.
+    -- (* maloc returned non-null value *)
+      forward.
+      unfold if_post1.
+      break_let.
+      Exists v.
+      Exists (snd p).
+      rewrite if_false by assumption.
+      repeat rewrite if_true by assumption.
+      entailer!.
+  * (* _st <> NULL *)
+    forward.
+    unfold if_post1.
+    Exists bv_p (map (fun x => Int.repr (Byte.unsigned x)) buf).
+    repeat rewrite if_false by assumption.
+    entailer!.  
+  * (* after the first if *)
+    unfold if_post1.
+    Intros p ls.
+    forward_empty_loop.
+    forward_call (ctx_p, ctx, td_p, td, nullval, nullval, buf_p, buf,
+                  v__res__1, size, tag_mode, 0, v_length, nullval, 0).
+    rewrite if_true in * by assumption.
+    pose proof Exec.ber_check_tags_bool_res td buf DT as BCT.
+    inversion BCT as [T | T]; rewrite T in *;
+        unfold construct_dec_rval, tag_length, tag_consumed.
+      2: { (* If ber_check_tags failed *)
+        normalize;
+        repeat forward.
+        all: forward_if; [|discriminate];
+          repeat forward.
+        Exists p ls.
+        inversion H0.
+        rewrite if_false by assumption.
+        unfold bool_decoder; rewrite T; 
+          destruct buf;  entailer!. 
+        simpl.
+        entailer!. }
+      (* If ber_check_tags succeded *)
+      { 
+        clear BCT; rename T into BCT; cbn in Size; subst.
+        normalize.
+        repeat forward.
+        forward_if; [congruence|].
+        forward_empty_loop.
+        repeat forward.
+        forward_if.
+        (* RW_MORE case *) admit.
+        forward.
+        forward_if True. 
+      (* if length <> 1 *)
+      (* Since we're not yet working with real type_descriptors we're assuming 
+         that if ber_check_tags succedes, then length = 1 *)
+        congruence.
+
+      forward; entailer!.
+      (* if length = 1 *)
+      cbn -[PROPx LOCALx SEPx abbreviate eq_dec nullval CompSpecs].
+      rewrite data_at_isptr with (p0 := buf_p).
+      normalize.
+      rewrite sem_add_pi_ptr.
+      2: assumption.
+      2: cbn; lia.
+      cbn -[PROPx LOCALx SEPx abbreviate eq_dec nullval CompSpecs]. 
+      assert_PROP (offset_val 2 buf_p = 
+                   field_address (tarray tuchar (Zlength buf)) 
+                                 [ArraySubsc 2] buf_p).
+      entailer!.
+      rewrite field_address_offset;
+      auto with field_compatible.
+      forward.
+      entailer!.
+      simpl. normalize.
+      rep_omega.
+      inversion H0.
+      assert (exists i, ls = [i]) as LS by admit. (* from H5 *)
+      destruct LS as [i LS].  
+      subst.  
+      Search tarray 1.
+      erewrite data_at_singleton_array_eq with (t := tint) (v := (Vint i)); auto.
+      Intros.
+      forward.
+      repeat forward.
+      forward_empty_loop.
+      repeat forward.
+      Exists p [i].
+      inversion H0.
+      rewrite if_false by assumption.
+      entailer!.
+      unfold bool_decoder; rewrite BCT; 
+        destruct buf; simpl; entailer!.
+      assert ((Zlength (i0 :: buf) - 2 <? 1) = false) as Z.
+      erewrite Z.ltb_ge.
+      nia.
+      rewrite Z.
+      destruct buf;
+      simpl;
+      simpl in H2;
+      try nia.
+      destruct buf.
+      simpl.
+      simpl in H2.
+      nia.
+      simpl.
+      entailer!.
+      cbn.
+      entailer!.
+      (* need to return byte and not bool *)
+      admit. }
+    - (* bv <> nullval *)
+  rename H0 into DT.
+  rename H1 into Size.
+  rename H2 into Len.
+  repeat forward.
+  forward_if (if_post1 bv_p v__res__1 v_tmp_error v_length v_rval res_p ctx 
+                       ctx_p td_p bv_pp buf buf_p size tag_mode).
+  congruence.
+  forward. 
+  unfold if_post1.
+   Exists bv_p (@nil int).
+   repeat rewrite if_false by assumption.
+   entailer!.
+  * (* after the first if *)
+    unfold if_post1.
+    Intros p ls.
+    forward_empty_loop.
+    forward_call (ctx_p, ctx, td_p, td, nullval, nullval, buf_p, buf,
+                  v__res__1, size, tag_mode, 0, v_length, nullval, 0). 
+    pose proof Exec.ber_check_tags_bool_res td buf DT as BCT.
+    inversion BCT as [T | T]; rewrite T in *;
+        unfold construct_dec_rval, tag_length, tag_consumed.
+      2: { (* If ber_check_tags failed *)
+           rewrite if_false by assumption.
+         normalize;
+        repeat forward.
+        all: forward_if; [|discriminate];
+          repeat forward.
+        unfold bool_decoder; rewrite T; 
+          destruct buf;  entailer!. 
+        simpl.
+        rewrite if_false in * by assumption.
+        inversion H0.
+        subst.
+        entailer!.
+      simpl. 
+      entailer!.
+       rewrite if_false in * by assumption.
+        inversion H0.
+        subst.
+        entailer!.
+      }
+      (* If ber_check_tags succeded *)
+      clear BCT; rename T into BCT; cbn in Size; subst.
+      normalize.
+      repeat forward.
+      forward_if; [congruence|].
+      forward_empty_loop.
+      repeat forward.
+      forward_if.
+      (* RW_MORE case *) admit.
+      forward.
+      forward_if True.
+      (* if length <> 1 *)
+      (* Since we're not yet working with real type_descriptors we're assuming 
+         that if ber_check_tags succedes, then length = 1 *)
+      congruence.
+
+      forward; entailer!.
+      (* if length = 1 *)
+      cbn -[PROPx LOCALx SEPx abbreviate eq_dec nullval CompSpecs].
+      rewrite data_at_isptr with (p0 := buf_p).
+      normalize.
+      rewrite sem_add_pi_ptr.
+      2: assumption.
+      2: cbn; lia.
+      cbn -[PROPx LOCALx SEPx abbreviate eq_dec nullval CompSpecs].
+      assert_PROP (offset_val 2 buf_p = 
+                   field_address (tarray tuchar (Zlength buf)) 
+                                 [ArraySubsc 2] buf_p).
+      entailer!.
+      rewrite field_address_offset;
+      auto with field_compatible.
+      forward.
+      entailer!.
+      simpl. normalize.
+      rep_omega.
+      rewrite if_false in * by assumption.
+      Intros.
+      inversion H0; subst.
+      repeat forward.
+      forward_empty_loop.
+      repeat forward.
+      unfold bool_decoder; rewrite BCT; 
+        destruct buf; simpl; entailer!.
+      assert ((Zlength (i :: buf) - 2 <? 1) = false) as Z.
+      erewrite Z.ltb_ge.
+      nia.
+      rewrite Z.
+      destruct buf;
+      simpl;
+      simpl in H2;
+      try nia.
+      destruct buf.
+      simpl.
+      simpl in H2.
+      nia.
+      simpl.
+      entailer!.
+      cbn.
+      entailer!.
+      (* need to return byte and not bool *)
+      admit.
+Admitted.
+
+(*
 Theorem bool_der_encode : semax_body Vprog Gprog 
            (normalize_function f_BOOLEAN_decode_ber composites) 
            bool_ber_decode_spec.
@@ -165,6 +412,7 @@ Proof.
     Exists bv_p (tptr tvoid) buf.
     repeat rewrite if_false by assumption.
     entailer!.
+    
   * (* after the first if *)
     unfold if_post1.
     Intros p t ls.
@@ -175,8 +423,9 @@ Proof.
     inversion BCT as [T | T]; rewrite T in *;
         unfold construct_dec_rval, tag_length, tag_consumed.
       2: { (* If ber_check_tags failed *)
-        repeat break_if;
-        normalize;
+        break_if.
+        (* p <> nullval *)
+        -  normalize;
         repeat forward.
         all: forward_if; [|discriminate];
           repeat forward.
@@ -186,10 +435,15 @@ Proof.
           destruct buf;  entailer!. 
         simpl.
         entailer!.
+        - (* bv_p <> nullval *)
+          Intros.
+          repeat forward.
+        all: forward_if; [|discriminate];
+          repeat forward.
         unfold bool_decoder. rewrite T.
         simpl.
-        destruct buf; inversion H0; entailer!. }
-
+        destruct buf; inversion H0; entailer!.
+      }
       (* If ber_check_tags succeded *)
       clear BCT; rename T into BCT; cbn in Size; subst.
       normalize.
@@ -224,10 +478,64 @@ Proof.
       forward.
       entailer!.
       admit.
-      break_if.
-      Intros.
-      Fail forward.
+      break_if. 
+      - Intros.
+        destruct ls.
+        simpl.
+        admit. 
+        assert (data_at Ews (tarray tuchar 1) (map Vubyte (i :: ls)) p
+             = data_at Ews tint (Vint (Int.repr (Byte.unsigned i))) p) as D by admit.
+        rewrite D.
+        repeat forward.
+        forward_empty_loop.
+        repeat forward.
+        Exists p t ls.
+        rewrite if_false by assumption.
+        entailer!.
+        unfold bool_decoder; rewrite BCT; 
+          destruct buf; simpl; entailer!.
+        replace  ((Zlength (i0 :: buf) - 2 <? 1) || false)%bool with false.
+        destruct buf.
+        simpl.
+        simpl in H2.
+        nia.
+        destruct buf.
+        simpl.
+        simpl in H2.
+        nia.
+        simpl.
+        entailer!.
+        cbn.
+        entailer!.
+        (* malloc precondition + tint tuchar issue *)
+        admit.
+        admit.
+      - (* bv_p <> nullval *)
+        Intros.
+        inversion H0; subst.
+        forward.
+         repeat forward.
+        forward_empty_loop.
+        repeat forward.
+        entailer!.
+         unfold bool_decoder; rewrite BCT; 
+          destruct buf; simpl; entailer!.
+          replace  ((Zlength (i :: buf) - 2 <? 1) || false)%bool with false.
+           destruct buf.
+        simpl.
+        simpl in H2.
+        nia.
+        destruct buf.
+        simpl.
+        simpl in H2.
+        nia.
+        simpl.
+        entailer!.
+        cbn.
+        entailer!.
+        admit.
+        admit.
 Admitted.
 
-
+*) 
 End Boolean_ber_decode.
