src/Lib/Stdlib.v
@@ -3,6 +3,24 @@ Require Import VST.floyd.proofauto.
 Require Import VST.floyd.library. (* contains malloc, exit and free specs *)
 
 Definition calloc_spec {cs : compspecs} :=
+   WITH m : Z, n : Z, t : type
+   PRE [ size_t, size_t ]
+       PROP (0 <= m <= Ptrofs.max_unsigned ;
+             0 <= n <= Ptrofs.max_unsigned ;
+             0 <= m * n <= Ptrofs.max_unsigned;
+             sizeof t = n)
+       PARAMS (Vptrofs (Ptrofs.repr m); 
+               Vptrofs (Ptrofs.repr n)) 
+       GLOBALS()
+       SEP ()
+    POST [ tptr tvoid ] EX p : val, EX ls : list int, 
+       PROP (Zlength ls = m;
+             Forall (fun x => x = Int.zero) ls)
+       LOCAL (temp ret_temp p)
+       SEP (if eq_dec p nullval then emp
+            else data_at Ews (tarray tint m) (map Vint ls) p).
+
+(* Definition calloc_spec {cs : compspecs} :=
    WITH m : Z, n : Z
    PRE [ size_t, size_t ]
        PROP (0 <= m <= Ptrofs.max_unsigned ;
@@ -12,13 +30,14 @@ Definition calloc_spec {cs : compspecs} :=
                Vptrofs (Ptrofs.repr n)) 
        GLOBALS()
        SEP ()
-    POST [ tptr tvoid ] EX p : val, EX t : type, EX ls : list byte, 
+    POST [ tptr tvoid ] EX p : val, EX ls : list byte, 
        PROP (Zlength ls = (m * n)%Z;
                Forall (fun x => x = Byte.zero) ls)
        LOCAL (temp ret_temp p)
        SEP (if eq_dec p nullval then emp
-            else malloc_token Ews t p * (* p is valid and malloc_compatible for t *)
-                  data_at Ews (tarray tschar m) (map Vbyte ls) p).
+            else (* malloc_token Ews (tarray tuchar m) p *
+                 (* p is valid and malloc_compatible for t *) *)
+                  data_at Ews (tarray tuchar m) (map Vubyte ls) p). *)
 
 Definition memcpy_spec {cs : compspecs} :=
     WITH qsh : share, psh: share, p: val, q: val, n: Z, contents: list int
